%%%%%%%%%%%%%%%%%%%%%%%%%%%%%%%%%%%%%%%%%%%%%%%%%%%%%%%%%%%%%%%%%%%%%%%%%%%%%%%%%%%%%%%%%%%%%%%%%%%%%%%%%%%%%%%%%%%%%%%%%%%%%%%%%%%%%%%%%%%%%%%%%%%%%%%%%%%%%%%%%%%%%%%%%%%%%%%%%%%%%%%%%%%%
% Written By Michael Brodskiy
% Class: Linear Algebra
% Professor: L. Knight
%%%%%%%%%%%%%%%%%%%%%%%%%%%%%%%%%%%%%%%%%%%%%%%%%%%%%%%%%%%%%%%%%%%%%%%%%%%%%%%%%%%%%%%%%%%%%%%%%%%%%%%%%%%%%%%%%%%%%%%%%%%%%%%%%%%%%%%%%%%%%%%%%%%%%%%%%%%%%%%%%%%%%%%%%%%%%%%%%%%%%%%%%%%%

\documentclass[12pt]{article} 
\usepackage{alphalph}
\usepackage[utf8]{inputenc}
\usepackage[russian,english]{babel}
\usepackage{titling}
\usepackage{amsmath}
\usepackage{graphicx}
\usepackage{enumitem}
\usepackage{amssymb}
\usepackage{physics}
\usepackage{tikz}
\usepackage{mathdots}
\usepackage{yhmath}
\usepackage{cancel}
\usepackage{color}
\usepackage{siunitx}
\usepackage{array}
\usepackage{multirow}
\usepackage{gensymb}
\usepackage{tabularx}
\usepackage{booktabs}
\usepackage{pifont}
\newcommand{\xmark}{\ding{55}}
\usetikzlibrary{fadings}
\usetikzlibrary{patterns}
\usetikzlibrary{shadows.blur}
\usetikzlibrary{shapes}
\usepackage[super]{nth}
\usepackage{expl3}
\usepackage[version=4]{mhchem}
\usepackage{hpstatement}
\usepackage{rsphrase}
\usepackage{everysel}
\usepackage{ragged2e}
\usepackage{geometry}
\usepackage{fancyhdr}
\usepackage{cancel}
\usepackage{multicol}
\geometry{top=1.0in,bottom=1.0in,left=1.0in,right=1.0in}
\newcommand{\subtitle}[1]{%
  \posttitle{%
    \par\end{center}
    \begin{center}\large#1\end{center}
    \vskip0.5em}%

}
\usepackage{hyperref}
\hypersetup{
colorlinks=true,
linkcolor=blue,
filecolor=magenta,      
urlcolor=blue,
citecolor=blue,
}

\urlstyle{same}


\title{Linear Algebra 6.3 Homework}
\date{}
\author{Michael Brodskiy\\ \small Instructor: Prof. Knight}

\begin{document}

\maketitle

\begin{enumerate}

    \begin{center}
      \underline{3, 5, 9, 15, 21, 37, 39, 42-49 odd, 51a}
    \end{center}

    \setcounter{enumi}{2}

  \item $\left\{\begin{array}{c} x+y\\x-y\\z-x\end{array}\Rightarrow\begin{bmatrix} 1 & 1 & 0\\ 1 & -1 & 0\\ -1 & 0 & 1\end{bmatrix}$

    \setcounter{enumi}{4}

  \item $\left\{\begin{array}{c} 3x-2z\\2y-z\end{array}\Rightarrow\begin{bmatrix} 3 & 0 & -2\\ 0 & 2 & -1  \end{bmatrix}$

    \setcounter{enumi}{8}

  \item $\begin{bmatrix} 1 & -3\\ 2 & 1\\ 0 & 1\end{bmatrix}\begin{bmatrix} -2\\4\end{bmatrix}=\begin{bmatrix} -14\\0\\4\end{bmatrix}\Rightarrow(-14,0,4)$

    \setcounter{enumi}{14}

  \item

    \begin{enumerate}

      \item  $\frac{1}{2}\begin{bmatrix} \sqrt{2} & -\sqrt{2}\\ \sqrt{2} & \sqrt{2} \end{bmatrix}$

      \item $\frac{1}{2}\begin{bmatrix} \sqrt{2} & -\sqrt{2}\\ \sqrt{2} & \sqrt{2} \end{bmatrix}\begin{bmatrix} 2\\2\end{bmatrix}=\begin{bmatrix} 0\\ 2\sqrt{2}\end{bmatrix}$

      \item Draw out a graph

    \end{enumerate}

    \setcounter{enumi}{20}

  \item

    \begin{enumerate}

      \item $\bold{w}\cdot\bold{w}=10\Rightarrow\frac{\bold{w}}{10}=\left( \frac{3}{10},\frac{1}{10} \right)\Rightarrow\begin{bmatrix} .9 & .3\\ .3 & .1\end{bmatrix}$

      \item $\begin{bmatrix} .9 & .3\\ .3 & .1\end{bmatrix}\begin{bmatrix} 1\\4\end{bmatrix}=\begin{bmatrix} \frac{21}{10}\\ \frac{7}{10} \end{bmatrix}$

      \item Draw out a graph

    \end{enumerate}

    \setcounter{enumi}{36}

  \item

    \begin{enumerate}

      \item $\begin{bmatrix} 1 & 1\\1 & 0\\ 0 &1  \end{bmatrix}\begin{bmatrix} 5\\4\end{bmatrix}=(9,5,4)$

      \item $T(1,-1)=(0,1,-1)\text{ and }T(0,1)=(1,0,1)\Rightarrow \begin{bmatrix} 0 & 1\\1 & 0\\-1 & 1\end{bmatrix}\begin{bmatrix} 5\\9\end{bmatrix}=\begin{bmatrix} 9\\5\\4\end{bmatrix}$

    \end{enumerate}

    \setcounter{enumi}{38}

  \item

    \begin{enumerate}

      \item $\begin{bmatrix}2 & 0 & 0\\ 1 & 1 & 0\\ 0 & 1 & 1\\ 1 & 0 & 1  \end{bmatrix}\begin{bmatrix} 1\\-5\\2\end{bmatrix}=\begin{bmatrix} 2\\-4\\-3\\3\end{bmatrix}$

      \item $T(2,0,1)=(4,2,1,3)\text{ and }T(0,2,1)=(0,2,3,1)\text{ and }T(1,2,1)=(2,3,3,2)\Rightarrow\begin{bmatrix} 4 & 0 & 2\\2 & 2 & 3\\ 1 & 3 & 3\\ 3  &1 & 2\end{bmatrix}\Rightarrow \left[ \begin{array}{ccc|c} 2 & 0 & 1 & 1\\ 0 & 2 & 2 & -5\\ 1 & 1 & 1 & 2  \end{array} \right]\widetilde{ }\left[ \begin{array}{ccc|c} 2 & 0 & 1 & 1\\ 0 & 1 & 1 & -\frac{5}{2}\\ 1 & 0 & 0 & \frac{9}{2}  \end{array} \right]\widetilde{ }\left[ \begin{array}{ccc|c} 1 & 0 & 0 & \frac{9}{2}\\ 0 & 1 & 0 & \frac{11}{2}\\ 0 & 0 & 1 & -8  \end{array} \right]\Rightarrow\begin{bmatrix} 4 & 0 &2\\ 2 & 2 &3\\ 1 & 3 & 3\\ 3&1 &2\end{bmatrix} \begin{bmatrix} \frac{9}{2}\\\frac{11}{2}\\-8\end{bmatrix}=\begin{bmatrix} 2\\-4\\-3\\3\end{bmatrix}$

    \end{enumerate}

    \setcounter{enumi}{42}

  \item $T(1)=x$, $T(x)=x^2$, $T(x^2)=x^3\Rightarrow\begin{bmatrix} 0 & 0 & 0\\ 1 & 0 & 0\\ 0 & 1 & 0\\ 0 & 0 & 1\end{bmatrix}$

    \setcounter{enumi}{44}

  \item $T(1)=0$, $T(x)=1$, $T(e^x)=e^x$, and $T(xe^x)=e^x+xe^x\Rightarrow\begin{bmatrix} 0 & 1 & 0 & 0\\ 0 & 0 & 0 & 0\\ 0 & 0 & 1 & 1\\ 0 & 0 & 1 & 0\end{bmatrix}$

    \setcounter{enumi}{46}

  \item $\begin{bmatrix} 0 & 1 & 0 & 0\\ 0 & 0 & 0 & 0\\ 0 & 0 & 1 & 1\\ 0 & 0 & 1 & 0\end{bmatrix}\begin{bmatrix} 0\\ 4\\ 0\\ -3\end{bmatrix}=\begin{bmatrix} 4\\ 0\\-3\\-3\end{bmatrix}=4-3e^x-3xe^x$

    \setcounter{enumi}{48}

  \item

    \begin{enumerate}

      \item $T(1)=x$, $T(x)=\frac{1}{2}x^2$, $T(x^2)=\frac{1}{3}x^3$, and $T(x^3)=\frac{1}{4}x^4\Rightarrow\begin{bmatrix} 0 & 0 & 0 & 0\\ 1 & 0 & 0 & 0\\ 0 & \frac{1}{2} & 0 & 0\\ 0 & 0 & \frac{1}{3} & 0\\ 0 & 0 & 0 & \frac{1}{4}  \end{bmatrix}$

      \item $\begin{bmatrix} 0 & 0 & 0 & 0\\ 1 & 0 & 0 & 0\\ 0 & \frac{1}{2} & 0 & 0\\ 0 & 0 & \frac{1}{3} & 0\\ 0 & 0 & 0 & \frac{1}{4}  \end{bmatrix}\begin{bmatrix} 8\\ -4\\0\\3\end{bmatrix}=\begin{bmatrix} 0\\8\\-2\\0\\\frac{3}{4}  \end{bmatrix}=8x-2x^2+\frac{3}{4}x^4$

    \end{enumerate}

    \setcounter{enumi}{50}

  \item $T\left( \begin{bmatrix} 1 & 0 & 0\\ 0 & 0 & 0 \end{bmatrix} \right)=\begin{bmatrix} 1 & 0\\0 & 0\\ 0 &0\end{bmatrix}$, $T\left( \begin{bmatrix} 0 & 1 & 0\\ 0 & 0 & 0 \end{bmatrix} \right)=\begin{bmatrix} 0 & 0\\1 & 0\\ 0 &0\end{bmatrix}$, $T\left( \begin{bmatrix} 0 & 0 & 1\\ 0 & 0 & 0 \end{bmatrix} \right)=\begin{bmatrix} 0 & 0\\0 & 0\\ 1 &0\end{bmatrix}$, $T\left( \begin{bmatrix} 0 & 0 & 0\\ 1 & 0 & 0 \end{bmatrix} \right)=\begin{bmatrix} 0 & 1\\0 & 0\\ 0 &0\end{bmatrix}$, $T\left( \begin{bmatrix} 0 & 0 & 0\\ 0 & 1 & 0 \end{bmatrix} \right)=\begin{bmatrix} 0 & 0\\0 & 1\\ 0 &0\end{bmatrix}$ $T\left( \begin{bmatrix} 0 & 0 & 0\\ 0 & 0 & 1 \end{bmatrix} \right)=\begin{bmatrix} 0 & 0\\0 & 0\\ 0 &1\end{bmatrix}$

    \begin{enumerate}

      \item $\begin{bmatrix} 1 & 0 & 0 & 0 & 0 & 0\\ 0 & 0 & 0 &1 & 0 & 0\\ 0 & 1 & 0 & 0 & 0 & 0\\ 0 & 0 & 0 & 0 & 1 & 0\\ 0 & 0 & 1 & 0 & 0 & 0\\ 0 & 0 & 0 & 0 & 0 & 1\end{bmatrix}$

    \end{enumerate}

\end{enumerate}

\end{document}

