%%%%%%%%%%%%%%%%%%%%%%%%%%%%%%%%%%%%%%%%%%%%%%%%%%%%%%%%%%%%%%%%%%%%%%%%%%%%%%%%%%%%%%%%%%%%%%%%%%%%%%%%%%%%%%%%%%%%%%%%%%%%%%%%%%%%%%%%%%%%%%%%%%%%%%%%%%%%%%%%%%%%%%%%%%%%%%%%%%%%%%%%%%%%
% Written By Michael Brodskiy
% Class: Linear Algebra (MATH-194)
% Professor: L. Knight
%%%%%%%%%%%%%%%%%%%%%%%%%%%%%%%%%%%%%%%%%%%%%%%%%%%%%%%%%%%%%%%%%%%%%%%%%%%%%%%%%%%%%%%%%%%%%%%%%%%%%%%%%%%%%%%%%%%%%%%%%%%%%%%%%%%%%%%%%%%%%%%%%%%%%%%%%%%%%%%%%%%%%%%%%%%%%%%%%%%%%%%%%%%%

\documentclass[12pt]{article} 
\usepackage{alphalph}
\usepackage[utf8]{inputenc}
\usepackage[russian,english]{babel}
\usepackage{titling}
\usepackage{amsmath}
\usepackage{graphicx}
\usepackage{enumitem}
\usepackage{amssymb}
\usepackage[super]{nth}
\usepackage{everysel}
\usepackage{ragged2e}
\usepackage{geometry}
\usepackage{fancyhdr}
\usepackage{cancel}
\usepackage{siunitx}
\geometry{top=1.0in,bottom=1.0in,left=1.0in,right=1.0in}
\newcommand{\subtitle}[1]{%
  \posttitle{%
    \par\end{center}
    \begin{center}\large#1\end{center}
    \vskip0.5em}%

}
\usepackage{hyperref}
\hypersetup{
colorlinks=true,
linkcolor=blue,
filecolor=magenta,      
urlcolor=blue,
citecolor=blue,
}

\urlstyle{same}


\title{Determinants \& Elementary Row Operations}
\date{\today}
\author{Michael Brodskiy\\ \small Professor: Lynn Knight}

% Mathematical Operations:

% Sum: $$\sum_{n=a}^{b} f(x) $$
% Integral: $$\int_{lower}^{upper} f(x) dx$$
% Limit: $$\lim_{x\to\infty} f(x)$$

\begin{document}

\maketitle

\begin{itemize}

  \item Let $\bold{A}$ and $\bold{B}$ be square matrices and $\bold{B}$ be a matrix resulting from $\bold{A}$ by:

    \begin{enumerate}

      \item interchanging two rows of $\bold{A}\Rightarrow\text{ det}(\bold{B})=-\text{ det}(\bold{A})$

      \item Multiplying row of $\bold{A}$ by a non-zero constant $\Rightarrow\text{ det}(\bold{B})=c\text{ det}(\bold{A})$, where $c$ is a scalar

      \item Add multiple of row of $\bold{A}$ to another row $\Rightarrow\text{ det}(\bold{B})=\text{ det}(\bold{A})$ (no change)

      \item ex. Given $\begin{vmatrix} a & b & c\\ d & e & f\\ g & h & i \end{vmatrix}=-6$

        \begin{enumerate}

          \item $\begin{vmatrix} d & e & f\\ a & b & c\\ g & h & i \end{vmatrix}=6$

          \item $\begin{vmatrix} 3a & 3b & 3c\\ 2d & 2e & 2f\\ -g & -h & -i \end{vmatrix}=-6(-6)=36$

          \item $\begin{vmatrix} a-d & b-e & c-f\\ 2d & 2e & 2f\\ g & h & i \end{vmatrix}=2(-6)=-12$

        \end{enumerate}

    \end{enumerate}

\end{itemize}

\end{document}

