%%%%%%%%%%%%%%%%%%%%%%%%%%%%%%%%%%%%%%%%%%%%%%%%%%%%%%%%%%%%%%%%%%%%%%%%%%%%%%%%%%%%%%%%%%%%%%%%%%%%%%%%%%%%%%%%%%%%%%%%%%%%%%%%%%%%%%%%%%%%%%%%%%%%%%%%%%%%%%%%%%%%%%%%%%%%%%%%%%%%%%%%%%%%
% Written By Michael Brodskiy
% Class: Linear Algebra
% Professor: L. Knight
%%%%%%%%%%%%%%%%%%%%%%%%%%%%%%%%%%%%%%%%%%%%%%%%%%%%%%%%%%%%%%%%%%%%%%%%%%%%%%%%%%%%%%%%%%%%%%%%%%%%%%%%%%%%%%%%%%%%%%%%%%%%%%%%%%%%%%%%%%%%%%%%%%%%%%%%%%%%%%%%%%%%%%%%%%%%%%%%%%%%%%%%%%%%

\documentclass[12pt]{article} 
\usepackage{alphalph}
\usepackage[utf8]{inputenc}
\usepackage[russian,english]{babel}
\usepackage{titling}
\usepackage{amsmath}
\usepackage{graphicx}
\usepackage{enumitem}
\usepackage{amssymb}
\usepackage{physics}
\usepackage{tikz}
\usepackage{mathdots}
\usepackage{yhmath}
\usepackage{cancel}
\usepackage{color}
\usepackage{siunitx}
\usepackage{array}
\usepackage{multirow}
\usepackage{gensymb}
\usepackage{tabularx}
\usepackage{booktabs}
\usepackage{pifont}
\newcommand{\xmark}{\ding{55}}
\usetikzlibrary{fadings}
\usetikzlibrary{patterns}
\usetikzlibrary{shadows.blur}
\usetikzlibrary{shapes}
\usepackage[super]{nth}
\usepackage{expl3}
\usepackage[version=4]{mhchem}
\usepackage{hpstatement}
\usepackage{rsphrase}
\usepackage{everysel}
\usepackage{ragged2e}
\usepackage{geometry}
\usepackage{fancyhdr}
\usepackage{cancel}
\usepackage{multicol}
\geometry{top=1.0in,bottom=1.0in,left=1.0in,right=1.0in}
\newcommand{\subtitle}[1]{%
  \posttitle{%
    \par\end{center}
    \begin{center}\large#1\end{center}
    \vskip0.5em}%

}
\usepackage{hyperref}
\hypersetup{
colorlinks=true,
linkcolor=blue,
filecolor=magenta,      
urlcolor=blue,
citecolor=blue,
}

\urlstyle{same}


\title{Linear Algebra 5.1 Homework}
\date{}
\author{Michael Brodskiy\\ \small Instructor: Prof. Knight}

\begin{document}

\maketitle

\begin{enumerate}

    \begin{center}
      \underline{Problems 1, 5, 9, 13, 17, 18, 21, 25, 27, 33, 41, 45, 49, 53, 57, 67, 71, 73, 77, 83, 84}
    \end{center}

  \item $\sqrt{3^2+4^2}=5$

    \setcounter{enumi}{4}

  \item

    \begin{enumerate}

      \item $\sqrt{\left( -1 \right)^2 + \left( \frac{1}{4} \right)^2}=\frac{\sqrt{17}}{4}$

      \item $\sqrt{\left( 4 \right)^2+\left( -\frac{1}{8} \right)^2}=\sqrt{\frac{1025}{64}}=\frac{5\sqrt{41}}{8}$

      \item $\sqrt{\left( -1+4 \right)^2+\left( \frac{1}{8} \right)^2}=\sqrt{\frac{577}{64}}=\frac{\sqrt{577}}{8}$

    \end{enumerate}

    \setcounter{enumi}{8}

  \item

    \begin{enumerate}

      \item $||\overrightarrow{u}||=13\Rightarrow\langle-\frac{5}{13},\frac{12}{13}\rangle$; $\left( -\frac{5}{13} \right)^2+\left( \frac{12}{13} \right)^2=1$

      \item Opposite Direction: $-\langle-\frac{5}{13},\frac{12}{13}\rangle=\langle\frac{5}{13},-\frac{12}{13}\rangle$; $\left( \frac{5}{13} \right)^2+\left( -\frac{12}{13} \right)^2=1$

    \end{enumerate}

    \setcounter{enumi}{12}

  \item $4\left( \langle1,1\rangle \right)\cdot\frac{1}{||\overrightarrow{u}||}=\langle2\sqrt{2},2\sqrt{2}\rangle$

    \setcounter{enumi}{16}

  \item

    \begin{enumerate}

      \item $\frac{1}{2}\overrightarrow{v}=\langle-\frac{1}{2},\frac{3}{2}, 0, 2\rangle$

      \item $-2\overrightarrow{v}=\langle2,-6,0,-8\rangle$

    \end{enumerate}

  \item $\sqrt{(c)^2+(2c)^2+(3c)^2}=1\Rightarrow c\sqrt{14}=\pm1\Rightarrow c=\frac{\sqrt{14}}{14}$

    \setcounter{enumi}{20}

  \item $\sqrt{(1-(-1))^2+(4-2)^2+(1-0)^2}=3$

    \setcounter{enumi}{24}

  \item

    \begin{enumerate}

      \item $\overrightarrow{u}\cdot\overrightarrow{v}=2(2)+(-1)(-2)+(-6)=0$

      \item $\overrightarrow{v}\cdot\overrightarrow{v}=(2)^2+(-1)^2+(-6)^2=41$

      \item $\left( \sqrt{(2)^2+(-2)^2+(1)^2 \right)^2=9$

      \item $(\overrightarrow{u}\cdot\overrightarrow{v})\overrightarrow{v}=\langle0,0\rangle$

      \item $\overrightarrow{u}\cdot(5\overrightarrow{v}}=5(\overrightarrow{u}\cdot\overrightarrow{v})=5(0)=0$

    \end{enumerate}

    \setcounter{enumi}{26}

  \item $(\overrightarrow{u}+\overrightarrow{v})\cdot(2\overrightarrow{u}-\overrightarrow{v})\Rightarrow2(\overrightarrow{u}\cdot\overrightarrow{u})-\overrightarrow{u}\cdot\overrightarrow{v}+2(\overrightarrow{u}\cdot\overrightarrow{v})-\overrightarrow{v}\cdot\overrightarrow{v}=2(4)-(-5)+2(-5)-(10)=-7$

    \setcounter{enumi}{32}

  \item

    \begin{enumerate}

      \item $||\overrightarrow{u}||\approx3.464$; $||\overrightarrow{v}||\approx3.317$

      \item $\langle-.603,.426,-.522,-.426\rangle$

      \item $\langle-.577,-.5,-.408,-.5\rangle$

      \item $-6.45$

      \item $12$

      \item $11$

    \end{enumerate}

    \setcounter{enumi}{40}

  \item $\theta=\cos^{-1}\left( \frac{\overrightarrow{u}\cdot\overrightarrow{v}}{||\overrightarrow{u}||||\overrightarrow{v}||} \right)$; $\overrightarrow{u}\cdot\overrightarrow{v}=\left( \frac{\sqrt{3}}{2} \right)\left( -\frac{\sqrt{2}}{2} \right)+\left( \frac{1}{2} \right)\left( \frac{\sqrt{2}}{2} \right)=\frac{-\sqrt{6}+\sqrt{2}}{4}$; $||\overrightarrow{u}||=\frac{5}{4}, ||\overrightarrow{v}||=\frac{3}{4}$; $\theta=106^{\circ}$

    \setcounter{enumi}{44}

  \item $||\overrightarrow{u}||=\sqrt{2}$, $||\overrightarrow{v}||=6$; $\overrightarrow{u}\cdot\overrightarrow{v}=6\Rightarrow\theta=\cos^{-1}\left( \frac{6}{6\sqrt{2}} \right)=45^{\circ}$

    \setcounter{enumi}{48}

  \item $-\frac{1}{3}(2)+\frac{2}{3}(-4)=-\frac{10}{3}\Rightarrow ||\overrightarrow{u}||=\frac{\sqrt{5}}{3}, ||\overrightarrow{v}||=2\sqrt{5}\Rightarrow\cos^{-1}(-1)=\pi$, so parallel

    \setcounter{enumi}{52}

  \item $\frac{1}{4}(-2)-\frac{5}{4}(5)=-\frac{27}{4}\Rightarrow ||\overrightarrow{u}||=\sqrt{30}, ||\overrightarrow{v}||=\sqrt{\frac{21}{8}}$, so neither

    \setcounter{enumi}{56}

  \item $2a-b+c=0\Rightarrow b=s, c=t\Rightarrow \langle \frac{s-t}{2},s,t\rangle$

    \setcounter{enumi}{66}

  \item

    \begin{enumerate}

      \item $\begin{bmatrix}3 & 4 \end{bmatrix}\begin{bmatrix}2\\-3 \end{bmatrix}=-6$

      \item $\begin{bmatrix} 2 & -3 \end{bmatrix} \begin{bmatrix} 2\\-3  \end{bmatrix}=13$

      \item $\begin{bmatrix} 3 & 4  \end{bmatrix} \begin{bmatrix} 3\\4  \end{bmatrix}=25$

      \item $\left(\begin{bmatrix}3 & 4 \end{bmatrix}\begin{bmatrix}2\\-3 \end{bmatrix}\right)\begin{bmatrix} 2 & -3\end{bmatrix}=\begin{bmatrix} -12 & 18 \end{bmatrix}$

      \item $\begin{bmatrix}3 & 4 \end{bmatrix}\left(5\begin{bmatrix}2\\-3 \end{bmatrix}\right)=5\left(\begin{bmatrix}3 & 4 \end{bmatrix}\begin{bmatrix}2\\-3 \end{bmatrix}\right)=-30$

    \end{enumerate}

    \setcounter{enumi}{70}

  \item $\overrightarrow{u}\cdot\overrightarrow{v}=(\cos\theta)(\sin\theta)+(\sin\theta)(-\cos\theta)=0$, so the two are orthogonal

    \setcounter{enumi}{72}

  \item

    \begin{enumerate}

      \item False. The norm is defined as the square root of the sum of all components squared.

      \item False. The dot product always becomes a scalar.

    \end{enumerate}

    \setcounter{enumi}{76}

  \item $v_1v_2+(v_2)(-v_1)=0$; $||\overrightarrow{v}||=13\Rightarrow\langle-\frac{12}{13},\frac{5}{13}\rangle,\langle\frac{12}{13},-\frac{5}{13}\rangle$

    \setcounter{enumi}{82}

  \item $\overrightarrow{u}\cdot(c\overrightarrow{v}+d\overrightarrow{w})=c(\overrightarrow{u}\cdot\overrightarrow{v})+d(\overrightarrow{u}\cdot\overrightarrow{w})=c(0)+d(0)=0$, so it is orthogonal

  \item $\overrightarrow{u}\cdot\overrightarrow{v}=\frac{1}{4}||\overrightarrow{u}+\overrightarrow{v}||^2-\frac{1}{4}||\overrightarrow{u}-\overrightarrow{v}||^2\Rightarrow \frac{1}{4}(\cancel{||\overrightarrow{u}||^2}+2(\overrightarrow{u}\cdot\overrightarrow{v})+\cancel{||\overrightarrow{v}||^2}\cancel{-||\overrightarrow{u}||^2}+2(\overrightarrow{u}\cdot\overrightarrow{v})\cancel{-||\overrightarrow{v}||^2})=\frac{1}{4}(4\overrightarrow{u}\cdot\overrightarrow{v})=\overrightarrow{u}\cdot\overrightarrow{v}\textcolor{green}{\checkmark}$

\end{enumerate}

\end{document}

